Work on packed/unpacked

DeBruijnSSA/BinSyntax/Rewrite/Region/Compose/Structural/Product.lean
@@ -20,7 +20,7 @@ theorem Eqv.unpacked_in_def' {Γ : Ctx α ε} {R : LCtx α} {r : Eqv φ [(Γ.pac
   ext k; cases k using Fin.elim1
   simp [Term.Subst.Eqv.get_comp]
 
-def Eqv.packed_in {Γ : Ctx α ε} {R : LCtx α} (r : Eqv φ Γ R) : Eqv φ [(Γ.pack, ⊥)] R
+def Eqv.packed_in {Γ : Ctx α ε} {R : LCtx α} (r : Eqv φ Γ R) : Eqv φ ((Γ.pack, ⊥)::Δ) R
   := r.vsubst Term.Subst.Eqv.unpack
 
 theorem Eqv.unpacked_in_packed_in {Γ : Ctx α ε} {R : LCtx α} {r : Eqv φ Γ R} {h : Γ.Pure}
@@ -32,7 +32,42 @@ theorem Eqv.packed_in_unpacked_in
   : (r.unpacked_in h).packed_in = r := by
   rw [unpacked_in_def', packed_in, vsubst_vsubst, Term.Subst.Eqv.unpack_comp_packSE, vsubst_id]
 
--- TODO: {br, let1, let2, case, cfg}
+open Term.Eqv
+
+-- TODO: br
+
+theorem Eqv.packed_in_let1 {Γ : Ctx α ε} {R : LCtx α}
+  {a : Term.Eqv φ Γ (A, e)} {r : Eqv φ ((A, ⊥)::Γ) R}
+  : (let1 a r).packed_in (Δ := Δ)
+  = let1 a.packed (let1 (pair (var 0 Ctx.Var.shead) (var 1 (by simp))) r.packed_in) := by
+  rw [packed_in, vsubst_let1]; apply congrArg
+  rw [packed_in, let1_beta, vsubst_vsubst, Term.Subst.Eqv.lift_unpack]
+
+theorem Eqv.packed_in_let2 {Γ : Ctx α ε} {R : LCtx α}
+  {a : Term.Eqv φ Γ (A.prod B, e)} {r : Eqv φ ((B, ⊥)::(A, ⊥)::Γ) R}
+  : (let2 a r).packed_in (Δ := Δ)
+  = let2 a.packed (let1
+    (pair (var 0 Ctx.Var.shead) (pair (var 1 (by simp)) (var 2 (by simp))))
+    r.packed_in) := by
+  rw [packed_in, vsubst_let2]; apply congrArg
+  rw [packed_in, let1_beta, vsubst_vsubst, Term.Subst.Eqv.liftn₂_unpack]
+
+theorem Eqv.packed_in_case {Γ : Ctx α ε} {R : LCtx α}
+  {a : Term.Eqv φ Γ (A.coprod B, e)} {r : Eqv φ ((A, ⊥)::Γ) R} {s : Eqv φ ((B, ⊥)::Γ) R}
+  : (case a r s).packed_in (Δ := Δ)
+  = case a.packed
+    (let1 (pair (var 0 Ctx.Var.shead) (var 1 (by simp))) r.packed_in)
+    (let1 (pair (var 0 Ctx.Var.shead) (var 1 (by simp))) s.packed_in) := by
+  rw [packed_in, vsubst_case]
+  congr <;> rw [packed_in, let1_beta, vsubst_vsubst, Term.Subst.Eqv.lift_unpack]
+
+theorem Eqv.packed_in_cfg {Γ : Ctx α ε} {R L : LCtx α}
+  {β : Eqv φ Γ (R ++ L)} {G}
+  : (cfg R β G).packed_in (Δ := Δ)
+  = cfg R β.packed_in (λi => (let1 (pair (var 0 Ctx.Var.shead) (var 1 (by simp))) (G i).packed_in))
+  := by
+  rw [packed_in, vsubst_cfg]; apply congrArg; funext i
+  rw [packed_in, let1_beta, vsubst_vsubst, Term.Subst.Eqv.lift_unpack]
 
 end Region
 
